nr: implementing methods for the flatcombiner
Signed-off-by: Reto Achermann <achreto@gmail.com>

concurrency/node-replication/FlatCombinerTokens.i.dfy
@@ -2,8 +2,10 @@ include "../framework/AsyncSSM.i.dfy"
 include "../../lib/Lang/NativeTypes.s.dfy"
 include "../../lib/Base/Option.s.dfy"
 include "Constants.i.dfy"
-include "../framework/Rw.i.dfy"
 include "FlatCombiner.i.dfy"
+include "../framework/Rw.i.dfy"
+include "../framework/GlinearMap.s.dfy"
+include "../framework/Ptrs.s.dfy"
 
 module FlatCombinerTokens {
   import opened RequestIds
@@ -11,19 +13,96 @@ module FlatCombinerTokens {
   import opened GhostLoc
   import opened Constants
   import opened Options
-  import opened FlatCombiner
+  import FC = FlatCombiner
+  import FCTokens = RwTokens(FC)
+  import GlinearMap
+  import Ptrs
 
   // Allows clients to enqueue requests
   // The combiner reads the requests and returns responses
   // This machinery allows us make sure the requestId of the request & response match
 
-  datatype FCClient = FCClient(ghost loc: Loc, ghost tid: nat, ghost state: FCClientState)
+  datatype {:glinear_fold} FCClient = FCClient(ghost loc: Loc, ghost tid: nat, ghost state: FC.FCClientState)
+  {
+    function defn(): FCTokens.Token {
+      FCTokens.T.Token(loc, FC.M(map[tid := state], map[], None))
+    }
+  }
 
-  datatype FCCombiner = FCCombiner(ghost loc: Loc, ghost state: FCCombinerState)
+  datatype {:glinear_fold}  FCCombiner = FCCombiner(ghost loc: Loc, ghost state: FC.FCCombinerState)
+  {
+    function defn(): FCTokens.Token {
+      FCTokens.T.Token(loc, FC.M(map[], map[], Some(state)))
+    }
+  }
 
-  datatype FCSlot = FCSlot(ghost loc: Loc, ghost tid: nat, ghost state: FCSlotState)
+  datatype {:glinear_fold} FCSlot = FCSlot(ghost loc: Loc, ghost tid: nat, ghost state: FC.FCSlotState)
+  {
+    function defn(): FCTokens.Token {
+      FCTokens.T.Token(loc, FC.M(map[], map[tid := state], None))
+    }
+  }
+
+
 
   // Ops for the combiner
+
+  // glinear method do_init_slots(glinear t: FCTokens.Token)
+  // returns (glinear slots: map<nat, FCSlot>)
+  // {
+  //   glinear var t' := t;
+  //   ghost var j := 0;
+  //   slots := GlinearMap.glmap_empty();
+
+  //   while j < MAX_THREADS_PER_REPLICA as nat
+  //   invariant 0 <= j <= LOG_SIZE as nat
+  //   invariant t'.loc == t.loc
+  //   invariant t'.val.M?
+  //   invariant forall i | 0 <= i < j :: i in slots && slots[i] == FCSlot(t.loc, j, FC.FCEmpty)
+  //   invariant forall i | j <= i <  MAX_THREADS_PER_REPLICA as nat :: t.val.slots[i] == t'.val.slots[i]
+  //   {
+  //     var expected := FCSlot(t.loc, j, FC.FCEmpty);
+  //     var x := expected.defn().val;
+  //     var y := t'.val.(slots := t'.val.slots - {j});
+
+  //     glinear var xl;
+  //     t', xl := FCTokens.T.split(t', y, x);
+
+  //     glinear var z := FCSlot_fold(expected, xl);
+  //     slots := GlinearMap.glmap_insert(slots, j, z);
+  //     j := j + 1;
+  //   }
+  //   Ptrs.dispose_anything(t');
+  // }
+
+  // glinear method do_init_clients(glinear t: FCTokens.Token)
+  // returns (glinear clients: map<nat, FCClient>)
+  // {
+  //   glinear var t' := t;
+  //   ghost var j := 0;
+  //   clients := GlinearMap.glmap_empty();
+
+  //   while j < MAX_THREADS_PER_REPLICA as nat
+  //   invariant 0 <= j <= LOG_SIZE as nat
+  //   invariant t'.loc == t.loc
+  //   invariant t'.val.M?
+  //   invariant forall i | 0<= i < j :: i in clients && clients[i] == FCClient(t.loc, i, FC.FCClientIdle)
+  //   invariant forall i | j <= i <  MAX_THREADS_PER_REPLICA as nat :: t.val.clients[i] == t'.val.clients[i]
+  //   {
+  //     var expected := FCClient(t.loc, j, FC.FCClientIdle);
+  //     var x := expected.defn().val;
+  //     var y := t'.val.(clients := t'.val.clients - {j});
+
+  //     glinear var xl;
+  //     t', xl := FCTokens.T.split(t', y, x);
+
+  //     glinear var z := FCClient_fold(expected, xl);
+  //     clients := GlinearMap.glmap_insert(clients, j, z);
+  //     j := j + 1;
+  //   }
+
+  //   Ptrs.dispose_anything(t');
+  // }
 
   glinear method fc_initialize()
   returns (
@@ -31,11 +110,35 @@ module FlatCombinerTokens {
     glinear slots: map<nat, FCSlot>,
     glinear combiner: FCCombiner
   )
-  ensures combiner.state == FCCombinerCollecting([])
+  ensures combiner.state == FC.FCCombinerCollecting([])
   ensures forall i | 0 <= i < MAX_THREADS_PER_REPLICA as int ::
-      i in slots && slots[i] == FCSlot(combiner.loc, i, FCEmpty)
+      i in slots && slots[i] == FCSlot(combiner.loc, i, FC.FCEmpty)
   ensures forall i | 0 <= i < MAX_THREADS_PER_REPLICA as int ::
-      i in clients && clients[i] == FCClient(combiner.loc, i, FCClientIdle)
+      i in clients && clients[i] == FCClient(combiner.loc, i, FC.FCClientIdle)
+  // {
+
+  //   ghost var new_clients := map x : nat | 0 <= x < (MAX_THREADS_PER_REPLICA as nat) :: x := FC.FCClientIdle;
+  //   ghost var new_slots   := map x : nat | 0 <= x < (MAX_THREADS_PER_REPLICA as nat) :: x := FC.FCEmpty;
+  //   ghost var new_comb := FC.FCCombinerCollecting([]);
+  //   ghost var m := FC.M(new_clients, new_slots, Some(new_comb));
+
+  //   FC.InitImpliesInv(m);
+  //   glinear var token := FCTokens.initialize_nonempty(0, m);
+
+  //   ghost var cl := FC.M(new_clients, map[], None);
+  //   ghost var s  := FC.M(map[], new_slots, None);
+  //   ghost var co := FC.M(map[], map[], Some(new_comb));
+
+  //   glinear var tcl, ts, tco := FCTokens.split3(token, cl, s, co);
+
+  //   clients := do_init_clients(tcl);
+  //   slots := do_init_slots(ts);
+  //   combiner := FCCombiner_fold(FCCombiner(token.loc, new_comb), tco);
+  // }
+
+  /* ----------------------------------------------------------------------------------------- */
+
+
 
   glinear method combiner_collect(glinear comb: FCCombiner, glinear slot: FCSlot)
   returns (glinear comb': FCCombiner, glinear slot': FCSlot)
@@ -46,19 +149,87 @@ module FlatCombinerTokens {
   ensures slot.state.FCEmpty? || slot.state.FCRequest?
   ensures slot.state.FCEmpty? ==>
       && comb' == FCCombiner(comb.loc,
-          FCCombinerCollecting(comb.state.elems + [None]))
+          FC.FCCombinerCollecting(comb.state.elems + [None]))
       && slot' == slot
   ensures slot.state.FCRequest? ==>
       && comb' == FCCombiner(comb.loc,
-          FCCombinerCollecting(
-            comb.state.elems + [Some(Elem(slot.state.rid))]))
-      && slot' == slot.(state := FCInProgress(slot.state.rid))
+          FC.FCCombinerCollecting(
+            comb.state.elems + [Some(FC.Elem(slot.state.rid))]))
+      && slot' == slot.(state := FC.FCInProgress(slot.state.rid))
+  {
+    glinear var c_token := FCCombiner_unfold(comb);
+    glinear var s_token := FCSlot_unfold(slot);
+
+    if slot.state.FCEmpty? {
+
+      ghost var out_expect_c := FCCombiner(comb.loc, FC.FCCombinerCollecting(comb.state.elems + [None]));
+      ghost var out_token_expect_c := FCCombiner_unfold(out_expect_c);
+
+      ghost var out_expect_s := FCSlot(slot.loc, slot.tid, FC.FCEmpty);
+      ghost var out_token_expect_s := FCSlot_unfold(out_expect_s);
+
+      FC.CombinerDoCollectEmpty_is_transition(
+        FC.dot(c_token.val, s_token.val),
+        FC.dot(out_token_expect_c.val, s_token.val)
+      );
+
+      glinear var out_token_c, out_token_s := FCTokens.internal_transition_2_2(
+        c_token, s_token, out_token_expect_c.val, s_token.val
+      );
+
+      comb' := FCCombiner_fold(out_expect_c, out_token_c);
+      slot' := FCSlot_fold(out_expect_s, out_token_s);
+
+    } else {
+
+      assume slot.state.FCRequest?;
+
+      ghost var out_expect_c := FCCombiner(comb.loc, FC.FCCombinerCollecting(comb.state.elems  + [Some(FC.Elem(slot.state.rid))]));
+      ghost var out_token_expect_c := FCCombiner_unfold(out_expect_c);
+
+      ghost var out_expect_s := FCSlot(slot.loc, slot.tid, FC.FCInProgress(slot.state.rid));
+      ghost var out_token_expect_s := FCSlot_unfold(out_expect_s);
+
+    FC.CombinerDoCollectRequest_is_transition(
+      FC.dot(c_token.val, s_token.val),
+      FC.dot(out_token_expect_c.val, out_token_expect_s.val)
+    );
+
+    glinear var out_token_c, out_token_s := FCTokens.internal_transition_2_2(
+      c_token, s_token, out_token_expect_c.val, out_token_expect_s.val
+    );
+
+    comb' := FCCombiner_fold(out_expect_c, out_token_c);
+    slot' := FCSlot_fold(out_expect_s, out_token_s);
+
+    }
+  }
+
+  /* ----------------------------------------------------------------------------------------- */
+
 
   glinear method combiner_goto_responding(glinear comb: FCCombiner)
   returns (glinear comb': FCCombiner)
   requires comb.state.FCCombinerCollecting?
   requires |comb.state.elems| == MAX_THREADS_PER_REPLICA as int
-  ensures comb' == FCCombiner(comb.loc, FCCombinerResponding(comb.state.elems, 0))
+  ensures comb' == FCCombiner(comb.loc, FC.FCCombinerResponding(comb.state.elems, 0))
+  {
+    glinear var c_token := FCCombiner_unfold(comb);
+
+    ghost var out_expect := FCCombiner(comb.loc, FC.FCCombinerResponding(comb.state.elems, 0));
+    ghost var out_token_expect := FCCombiner_unfold(out_expect);
+
+    FC.CombinerGoToResponding_is_transition(c_token.val,out_token_expect.val);
+
+    glinear var out_token := FCTokens.internal_transition(c_token, out_token_expect.val);
+
+    comb' := FCCombiner_fold(out_expect, out_token);
+
+  }
+
+
+  /* ----------------------------------------------------------------------------------------- */
+
 
   glinear method combiner_response_skip(glinear comb: FCCombiner)
   returns (glinear comb': FCCombiner)
@@ -66,6 +237,23 @@ module FlatCombinerTokens {
   requires comb.state.idx < |comb.state.elems|
   requires comb.state.elems[comb.state.idx].None?
   ensures comb' == FCCombiner(comb.loc, comb.state.(idx := comb.state.idx + 1))
+  {
+    glinear var c_token := FCCombiner_unfold(comb);
+
+    ghost var out_expect := FCCombiner(comb.loc, FC.FCCombinerResponding(comb.state.elems, comb.state.idx + 1));
+    ghost var out_token_expect := FCCombiner_unfold(out_expect);
+
+
+    FC.CombinerDoResponseSkip_is_transition(c_token.val,out_token_expect.val);
+
+    glinear var out_token := FCTokens.internal_transition(c_token, out_token_expect.val);
+
+    comb' := FCCombiner_fold(out_expect, out_token);
+  }
+
+
+  /* ----------------------------------------------------------------------------------------- */
+
 
   glinear method combiner_respond(glinear comb: FCCombiner, glinear slot: FCSlot)
   returns (glinear comb': FCCombiner, glinear slot': FCSlot)
@@ -76,14 +264,65 @@ module FlatCombinerTokens {
   requires comb.loc == slot.loc
   ensures slot.state.FCInProgress?
   ensures comb' == FCCombiner(comb.loc, comb.state.(idx := comb.state.idx + 1))
-  ensures slot' == slot.(state := FCResponse(slot.state.rid))
+  ensures slot' == slot.(state := FC.FCResponse(slot.state.rid))
   ensures comb.state.elems[comb.state.idx].value.rid == slot.state.rid
+  {
+    // that should follow from the invariant, need to obtain the invariant here.
+    assume slot.state.FCInProgress?;
+    assume comb.state.elems[comb.state.idx].value.rid == slot.state.rid;
+
+
+    glinear var c_token := FCCombiner_unfold(comb);
+    glinear var s_token := FCSlot_unfold(slot);
+
+    ghost var out_expect_c := FCCombiner(comb.loc, FC.FCCombinerResponding(comb.state.elems, comb.state.idx + 1));
+    ghost var out_token_expect_c := FCCombiner_unfold(out_expect_c);
+
+    ghost var out_expect_s := FCSlot(slot.loc, slot.tid, FC.FCResponse(slot.state.rid));
+    ghost var out_token_expect_s := FCSlot_unfold(out_expect_s);
+
+    FC.CombinerDoResponse_is_transition(
+      FC.dot(c_token.val, s_token.val),
+      FC.dot(out_token_expect_c.val, out_token_expect_s.val)
+    );
+
+    glinear var out_token_c, out_token_s := FCTokens.internal_transition_2_2(
+      c_token, s_token, out_token_expect_c.val, out_token_expect_s.val
+    );
+
+    comb' := FCCombiner_fold(out_expect_c, out_token_c);
+    slot' := FCSlot_fold(out_expect_s, out_token_s);
+  }
+
+
+  /* ----------------------------------------------------------------------------------------- */
+
 
   glinear method combiner_goto_collecting(glinear comb: FCCombiner)
   returns (glinear comb': FCCombiner)
   requires comb.state.FCCombinerResponding?
   requires comb.state.idx == MAX_THREADS_PER_REPLICA as int
-  ensures comb' == FCCombiner(comb.loc, FCCombinerCollecting([]))
+  ensures comb' == FCCombiner(comb.loc, FC.FCCombinerCollecting([]))
+  {
+    glinear var c_token := FCCombiner_unfold(comb);
+
+    // that can be obtained from the Invariant: CombinerState_Elems
+    assume |comb.state.elems| == MAX_THREADS_PER_REPLICA as int;
+
+    ghost var out_expect := FCCombiner(comb.loc, FC.FCCombinerCollecting([]));
+    ghost var out_token_expect := FCCombiner_unfold(out_expect);
+
+
+    FC.CombinerGoToCollecting_is_transition(c_token.val,out_token_expect.val);
+
+    glinear var out_token := FCTokens.internal_transition(c_token, out_token_expect.val);
+
+    comb' := FCCombiner_fold(out_expect, out_token);
+  }
+
+
+  /* ----------------------------------------------------------------------------------------- */
+
 
   // Ops for the requester
 
@@ -93,8 +332,40 @@ module FlatCombinerTokens {
   requires fc_client.tid == fc_slot.tid
   requires fc_client.state.FCClientIdle?
   ensures fc_slot.state.FCEmpty?
-  ensures fc_client' == fc_client.(state := FCClientWaiting(rid))
-  ensures fc_slot' == fc_slot.(state := FCRequest(rid))
+  ensures fc_client' == fc_client.(state := FC.FCClientWaiting(rid))
+  ensures fc_slot' == fc_slot.(state := FC.FCRequest(rid))
+  {
+    // that should follow from the invariant
+    assume fc_slot.state.FCEmpty?;
+
+    glinear var c_token := FCClient_unfold(fc_client);
+    glinear var s_token := FCSlot_unfold(fc_slot);
+
+    ghost var out_expect_c := FCClient(fc_client.loc, fc_client.tid , FC.FCClientWaiting(rid));
+    ghost var out_token_expect_c := FCClient_unfold(out_expect_c);
+
+    ghost var out_expect_s := FCSlot(fc_slot.loc, fc_slot.tid, FC.FCRequest(rid));
+    ghost var out_token_expect_s := FCSlot_unfold(out_expect_s);
+
+
+    FC.FCSend_is_transition(
+      FC.dot(c_token.val, s_token.val),
+      FC.dot(out_token_expect_c.val, out_token_expect_s.val),
+      fc_client.tid,
+      rid
+    );
+
+    glinear var out_token_c, out_token_s := FCTokens.internal_transition_2_2(
+      c_token, s_token, out_token_expect_c.val, out_token_expect_s.val
+    );
+
+    fc_client':= FCClient_fold(out_expect_c, out_token_c);
+    fc_slot'  := FCSlot_fold(out_expect_s, out_token_s);
+  }
+
+
+  /* ----------------------------------------------------------------------------------------- */
+
 
   glinear method fc_recv(glinear fc_client: FCClient, glinear fc_slot: FCSlot, ghost rid: RequestId)
   returns (glinear fc_client': FCClient, glinear fc_slot': FCSlot)
@@ -105,12 +376,44 @@ module FlatCombinerTokens {
   requires !fc_slot.state.FCInProgress?
   ensures fc_slot.state.FCResponse?
   ensures fc_slot.state.rid == fc_client.state.rid
-  ensures fc_client' == fc_client.(state := FCClientIdle)
-  ensures fc_slot' == fc_slot.(state := FCEmpty)
+  ensures fc_client' == fc_client.(state := FC.FCClientIdle)
+  ensures fc_slot' == fc_slot.(state := FC.FCEmpty)
+  {
+    // that should follow from the invariant
+    assume fc_slot.state.FCResponse?;
+    assume fc_slot.state.rid == fc_client.state.rid;
+
+    glinear var c_token := FCClient_unfold(fc_client);
+    glinear var s_token := FCSlot_unfold(fc_slot);
+
+    ghost var out_expect_c := FCClient(fc_client.loc, fc_client.tid , FC.FCClientIdle);
+    ghost var out_token_expect_c := FCClient_unfold(out_expect_c);
+
+    ghost var out_expect_s := FCSlot(fc_slot.loc, fc_slot.tid, FC.FCEmpty);
+    ghost var out_token_expect_s := FCSlot_unfold(out_expect_s);
+
+
+    FC.FCRecv_is_transition(
+      FC.dot(c_token.val, s_token.val),
+      FC.dot(out_token_expect_c.val, out_token_expect_s.val),
+      fc_client.tid,
+      rid
+    );
+
+    glinear var out_token_c, out_token_s := FCTokens.internal_transition_2_2(
+      c_token, s_token, out_token_expect_c.val, out_token_expect_s.val
+    );
+
+    fc_client':= FCClient_fold(out_expect_c, out_token_c);
+    fc_slot'  := FCSlot_fold(out_expect_s, out_token_s);
+  }
+
+  /* ----------------------------------------------------------------------------------------- */
+
 
   //// Utilties for the impl
 
-  predicate RidsMatch(bools: seq<Option<Elem>>, rids: seq<RequestId>,
+  predicate RidsMatch(bools: seq<Option<FC.Elem>>, rids: seq<RequestId>,
       bools_start: nat,
       bools_end: nat,
       rids_start: nat,
@@ -132,7 +435,7 @@ module FlatCombinerTokens {
     )
   }
 
-  lemma {:induction true} RidsMatchAddNone(bools: seq<Option<Elem>>, rids: seq<RequestId>,
+  lemma {:induction true} RidsMatchAddNone(bools: seq<Option<FC.Elem>>, rids: seq<RequestId>,
       bools_start: nat,
       bools_end: nat,
       rids_start: nat,
@@ -144,7 +447,7 @@ module FlatCombinerTokens {
   {
   }
 
-  lemma {:induction true} RidsMatchAddRidElem(bools: seq<Option<Elem>>, rids: seq<RequestId>,
+  lemma {:induction true} RidsMatchAddRidElem(bools: seq<Option<FC.Elem>>, rids: seq<RequestId>,
       bools_start: nat,
       bools_end: nat,
       rids_start: nat,
@@ -153,11 +456,11 @@ module FlatCombinerTokens {
   requires 0 <= bools_start <= bools_end <= |bools|
   requires 0 <= rids_start <= rids_end <= |rids|
   requires RidsMatch(bools, rids, bools_start, bools_end, rids_start, rids_end)
-  ensures RidsMatch(bools+[Some(Elem(rid))], rids+[rid], bools_start, bools_end, rids_start, rids_end)
+  ensures RidsMatch(bools+[Some(FC.Elem(rid))], rids+[rid], bools_start, bools_end, rids_start, rids_end)
   {
   }
 
-  lemma RidsMatchPop(bools: seq<Option<Elem>>, rids: seq<RequestId>,
+  lemma RidsMatchPop(bools: seq<Option<FC.Elem>>, rids: seq<RequestId>,
       bools_start: nat,
       bools_end: nat,
       rids_start: nat,
